\documentclass[12pt]{article} 

\usepackage{amsmath, amssymb, amsthm}
\usepackage{enumitem}
\usepackage{titlesec}

\titleformat{\section}[block]{\normalfont\LARGE\bfseries\centering}{\thesection}{1em}{}
\titleformat{\subsection}[runin]{\normalfont\Large\bfseries}{\thesubsection}{1em}{}

\usepackage[a4paper, top=2.5cm, bottom=2.5cm, left=3cm, right=3cm]{geometry}

\usepackage{setspace}
\setstretch{1.25}              
\setlength{\parskip}{5pt}     
\setlength{\parindent}{0em} 

\usepackage{fancyhdr}
\setlength{\headheight}{16pt}
\pagestyle{fancy}
\fancyhf{}
\fancyhead[C]{\nouppercase{\leftmark}} 
\fancyfoot[C]{\thepage}                
\renewcommand{\headrulewidth}{0.4pt}
\renewcommand{\footrulewidth}{0pt}

\newtheoremstyle{oneline}% name
  {}% space above
  {}% space below
  {\normalfont}% body font
  {}% indent amount
  {\bfseries}% theorem head font
  {}% punctuation after theorem head
  {0.6em}% space after theorem head
  {\thmname{#1}\thmnumber{ #2}\thmnote{\textit{ (#3)}}}
\theoremstyle{oneline}

\newtheorem{theorem}{Theorem}[subsection]
\newtheorem{lemma}{Lemma}[subsection]
\newtheorem{remark}{Remark}[subsection]
\newtheorem{proposition}{Proposition}[subsection]
\newtheorem{corollary}{Corollary}[subsection]
\newtheorem{definition}{Definition}[subsection]
\newtheorem{example}{Example}[subsection]
\newtheorem{property}{Property}[subsection]

\newtheoremstyle{twoline}% name
  {1em}% space above
  {0.5em}% empace below
  {\rmfamily}% body font
  {}% indent amount
  {\bfseries}% theorem head font
  {}% punctuation after theorem head
  {\newline}% space after theorem head
  {\large\thmname{#1}}
\theoremstyle{twoline}
\newtheorem{introduction}{Introduction}
\newtheorem{exercise}{Exercise}[section]

\makeatletter 
\@addtoreset{equation}{section}
\makeatother
\renewcommand{\theequation}{\thesection.\arabic{equation}}


\title{Mathematical Analysis Study Notes}
\author{Emrys}
\date{}

\begin{document} 
\maketitle
\tableofcontents
\newpage

\section{Numerical Sequences and Series}

\subsection{Series}
\begin{definition}
  Given a sequence $\{a_n\}$,we use the notation
   \[\sum\limits_{n=p}^{q}a_n\quad (p\leq q)\]
  to denote the sum $a_p+a_{p+1}+\cdots+a_q$. And we call the symbolic expression
  \[\sum\limits_{n=1}^{\infty}a_n=a_1+a_2+\cdots+a_n+\cdots\]
  an infinite series, or just a series.

  With $\{a_n\}$ we associate a sequence $\{S_n\}$, where
  \[S_n=\sum\limits_{k=1}^n a_k.\]
  The numbers $S_n$ are called the partial sums of the series.

  If $\{S_n\}$ converges to $s$, we say that the series converges, and write
  \[\sum\limits_{n=1}^{\infty}a_n=s.\]
  The number $s$ is called the sum of seires; If $\{S_n\}$ diverges, the series is said to diverge.
\end{definition}

\begin{remark}
  The above $s$ is called the sum of the series; but it should be clearly understood that s is the limit of a sequence of sums, and is not obtained simply by addition.
\end{remark}

\begin{remark}
  It is clear that every theorem about sequences can be state in series. The Cauchy criterion can be restated in the following form. 
\end{remark}

\begin{remark}
  For convenience of notation, we shall simply write $\Sigma a_n$ in place of $\sum\limits_{n=1}^{\infty}$.
\end{remark}

\begin{theorem}[Cauchy criterion]
  $\Sigma a_n$ converges $\iff$ for every $\varepsilon>0$ there exists an integer $N$ such that if $m\geq n\geq M$
  \begin{align}
    |\sum\limits_{k=n}^m a_k|\leq \varepsilon
  \end{align}
  It can be poved by the Cauchy criterion of the limit of sequences.
  And In particular, by taking $m=n$, $(\thesection.1)$ becomes
  \[|a_n|\leq\varepsilon\quad(n\geq N).\]
  So we can get the following vanishing condition.
\end{theorem}

\begin{theorem}[Vanishing condition]
  If $\Sigma a_n$ converges, then $\lim\limits_{n\to\infty}a_n=0$.
\end{theorem}

\begin{remark}
  The condition $a_n\to0$ is not, however, sufficient to ensure convergence of $\Sigma a_n$. For instance, the series 
  \[\sum\limits_{n=1}^\infty \frac1n\]
  diverges;and we will prove it in the \textit{Example \thesubsection.2}.
\end{remark}

\begin{example}
  let $q\in\mathbb{R}$, discuss the convergence and divergence of the geometric series $\Sigma q^n$.\\
\textit{Solution:} We know that the partial sum of it is $S_n=\frac{q(1-q^n)}{1-q}$, so we have the series converges when $|q|<1$ and diverges when $|q|\geq1$.
\end{example}

\begin{example}
  Determine the convergence and divergence of the harmonic series $\Sigma \frac1n$.\\
  \textit{Solution:} When $n\geq 1$, we have
  \[\sum\limits_{k=n+1}{2n}\frac1k\geq\sum\limits_{k=n+1}{2n}\frac1{2n}=\frac12,\]
  so by Cauchy criterion, we know the original series diverges.
\end{example}

\subsection{Positive Series}
\introduction
\hspace*{2em}
When studying a subject, we usually proceed from the specific to the general. Therefore, when researching series, we first focus on a specific type of series. It is called the positive series, which, as the name suggests, are series where each term is a positive number. But next, we will also reseach the non-negetive series meanwhile.

\begin{theorem}[Fundamental Test]
  The positive series converges $\iff$ $\{S_n\}$ is bounded above.

\textit{Proof:} Because $a_n>0$, We conclude that this partial sum $S_n$ is monotonically increasing with respect to $n$. It follows from the fact that a monotonically increasing and bounded above sequence must converge that $\{S_n\}$ converges.
\end{theorem}

\begin{remark}
  The above test also holds for $a_n\geq0$.
\end{remark}

\begin{theorem}[Cauchy Condensation Test]
  Suppose $a_1\geq a_2\geq a_3\geq\cdots\geq0$. Then the series $\sum\limits_{n=1}^{\infty} a_n$ converges if and only if the series $\sum\limits_{k=0}^\infty 2^ka_{2^k}$ converges.

\textit{Proof:} By the \textit{Theorem \thesubsection.1}, it suffices to consider boundness of the partial sums. let
\begin{align*}
  S_n=\sum\limits_{k=1}^n&=a_1+a_2+\cdots+a_n,\\
  T_m=\sum\limits_{k=0}^m2^ka^{2^k}&=a_1+2a_2+\cdots+2^ma_{2^m}
\end{align*}
When $2^m\leq n\leq 2^{m+1}$, we have
\begin{align*}
  S_n&\leq a_1+(a_2+a_3)+\cdots+(a_{2^m}+\cdots+a_{2^{m+1}-1})\\ 
  &\leq a_1+2a_2+\cdots+2^ma^{2^m}=T_m
\end{align*}
and 
\begin{align*}
  S_n&\geq a_1+a_2+(a_3+a_4)+\cdots+(a_{2^{m-1}+1}+\cdots+a_{2^m})\\
  &\geq \frac12 a_1+a_2+2a_4+\cdots+2^{m-1}a_{2^m}=\frac12T_m
\end{align*}
Thus, we have $S_n$ is bounded above $\iff$ $T_m$ is abounded above. This completes the proof.
\end{theorem}

\begin{example}
  $\Sigma \frac1{n^p}$ converges if $p>1$ and diverges if $p\leq 1$.

\textit{Proof:} If $p\leq 0$, divergence follows from the vanishing condition of series. \\
If $p>0$, \textit{Theorem \thesubsection.2} is applicable, we are led to the series 
\[\sum\limits_{k=0}^{\infty}2^k\cdot\frac1{2^{kp}}=\sum\limits_{k=0}^{\infty}2^{(1-p)k}=\sum\limits_{k=0}^{\infty}(2^{1-p})^k.\]
Now, $|2^{1-p}|<1\iff p>1$, and the proof follows by the first example of the previous subsection.
\end{example}

\begin{example}
  $\sum\limits_{n=2}^{\infty} \frac1{n(\ln n)^p}$ converges if $p>1$ and diverges if $p\leq 1$.

\textit{Proof:} We consider the series 
\[\sum\limits_{k=1}^{\infty}2^k\cdot\frac1{2^k(\ln 2^k)^p}=(\ln 2)^{-p}\sum\limits_{k=1}^\infty\frac1{k^p}\]
By \textit{Example \thesubsection.2}, we can easily prove the original proposition.
\end{example}

\begin{corollary}
  The above procedure may evidently be continued. In other words, we can also conclude 
  \[\sum\limits_{n=3}^\infty\frac1{n\ln n(\ln(\ln n))^p}\] converges if and only if $p>1$, and so forth. For instance,
  \begin{align}
    \sum\limits_{n=3}^\infty\frac1{n\ln n(\ln(\ln n))} 
  \end{align}
  diverges, whreas
  \begin{align}
    \sum\limits_{n=3}^\infty\frac1{n\ln n(\ln(\ln n))^2}
  \end{align}
  converges.
\end{corollary}

\begin{introduction}
  \hspace*{2em}
  From the above corollary, we may now observe that the series $(\thesection.2)$ differ very little from those of $(\thesection.3)$. Still, one diverges, and the other converges. If we continue the process which led us from \textit{Example \thesubsection.1} to \textit{Example \thesubsection.2}, and then to $(\thesection.2)$ and $(\thesection.3)$, we also get pairs of convergent and divergent series whose terms differ even less than those of $(\thesection.2)$ and $(\thesection.3)$.\\
  \hspace*{2em}
  Thus, one might be led to the conjecture that there is a limiting situation of some sort, i.e. a "boundary" with all convergent series on one side, all divergent series on the other side.
  Or when n is sufficiently large, Is there a largest convergent series?\\
  \hspace*{2em}
  In the following, We shall show that this conjecture is false.
\end{introduction}

\begin{proposition}
  Suppose positive seires $\Sigma a_n$ converges, then there must exist positive series $\Sigma b_n$ converges and satisfies $\lim\limits_{n\to\infty}\frac{b_n}{a_n}=+\infty$.

\textit{Proof:} Let 
\[S_n=a_1+\cdots+a_n,\]
\[T_n=a_n+a_{n+1}+\cdots=\sum\limits_{k=n}^\infty a_k.\]
We initially prove that $S_n$ converges $\iff$ $T_n$ converges to $0$. We can easily prove that $T_n$ converges iff $T_n$ converges to $0$. Hence, next we use the Cauchy criterion to prove
\[S_n ~converges \iff T_n~ converges.\]
Since for $m>n$,
\[T_m-T_n=a_n+\cdots+a_{m-1}=S_{m-1}-S_{n-1}\]
So we have for every $\varepsilon>0$, there exists $N_1>0$, such that for $m>n>N$, $|T_m-T_n|<\varepsilon$, if and only if for every $\varepsilon>0$, there exists $N_1>0$, such that for $m>n>N$, $|S_m-S_n|<\varepsilon$.
In other words, the above proposition holds.\\
By
\[a_n=T_n-T_{n+1}=(\sqrt{T_n}-\sqrt{T_{n+1}})(\sqrt{T_n}+\sqrt{T_{n+1}}),\]
we set $b_n=\sqrt{T_n}-\sqrt{T_{n+1}}$, and $B_n=\Sigma b_n=\sqrt{T_1}-\sqrt{T_n+1}$.\\
Hence, $\Sigma b_n$ converges owing to the convergence of $T_n$, and we have 
\[\frac{b_n}{a_n}=\frac1{\sqrt{T_n}+\sqrt{T_{n+1}}}\to \infty,\quad (n\to \infty)\]
\end{proposition}

\introduction
\hspace*{2em}
From the proof of \textit{Theorem \thesubsection.2}, we can know that for the non-negetive series $\Sigma a_n, \Sigma b_n$, if $A_n\leq B_n$ and $\Sigma b_n$ converges, then $\Sigma a_n$ converges.\\
\hspace*{2em}
This is rooted from the \textit{Theorem \thesubsection.1}, we can expand this to more general case.

\begin{theorem}[Comparison Test]
  Suppose $\Sigma a_n, \Sigma b_n$ are non-negetive series, if there exists $C>0, N\geq1$, such that $a_n\leq Cb_n$ for $n>N$, then if $\Sigma b_n$ converges, $\Sigma a_n$ also converges and if $\Sigma a_n$ diverges, $\Sigma b_n$ also diverges.
\end{theorem}

\begin{remark}
  Whether analyzing a single series or comparing two series, we actually don't need to consider the finite initial terms. That is to say, we can only consider the case when n is sufficiently large, and we can even remove the finite terms from one series to compare it with another series.
\end{remark}

\subsection{The Root and Ratio Tests}
\begin{introduction}
  \hspace*{2em}
  The above comparison test could generate other useful tests if we let $b$ be some series whose convergence or divergence is known.\\
  \hspace*{2em} 
  Sometimes if we cannot find some series which have some relationship with the original series, we can try some typical series like $\Sigma q^n, \Sigma \frac1{n^q}, \Sigma \frac1{n\ln n} $
\end{introduction}

\end{document}
